CombinatoryLogicAlgebra.v
@@ -7,6 +7,7 @@ Require Import Coq.Arith.PeanoNat.
 Require Import CombinatoryLogic.
 Require Import ComputationalPathLemma.
 Require Import IntersectionTypes.
+Require Import CombinatoryTerm.
 Require Import SigmaAlgebra.
 Require Import Cantor.
 
@@ -25,8 +26,114 @@ Module Type CompatibleCLSignature <: SignatureWithCLSig.
   Declare Instance Variables_finite: Finite VariableSymbol.
   Parameter ClosedSortsInhabited: Sort EmptySet.
   Parameter OpenSortsInhabited: Sort Var.
-End CompatibleCLSignature.
+  Parameter BlackBox : ConstructorSymbol.
+  Parameter BlackBoxArity: constructorArity BlackBox = 1.
+End CompatibleCLSignature.  
+
+
+Module Type SortEmbedding(Import SigSpec: CompatibleCLSignature)(Import Types: IntersectionTypes(SigSpec)).
+  Class Embedding (A: Set) :=
+    { embed: Sort A -> TypeScheme (VariableSymbol := A);
+      unembed: TypeScheme (VariableSymbol := A) -> Sort A; }.
+
+  Definition embedSubst `{Embedding EmptySet}: (SigSpec.Var -> Sort EmptySet) -> (SigSpec.Var -> IntersectionType) :=
+    fun S alpha => freeze (embed (S alpha)).
+  Definition unembedSubst `{Embedding EmptySet}: (SigSpec.Var -> IntersectionType) -> (SigSpec.Var -> Sort EmptySet) :=
+    fun S alpha => unembed (unfreeze (S alpha)).
+
+  Class InjectiveEmbedding (A: Set) :=
+    { Embed :> Embedding A;
+      unembedEmbed: forall (s: Sort A), unembed (embed s) = s }.
+
+  Lemma embedUnembed:
+    forall {A: Set} `{InjectiveEmbedding A} (ty: TypeScheme (VariableSymbol := A)),
+    (forall (sigma tau: TypeScheme (VariableSymbol := A)), { sigma = tau } + { sigma <> tau }) ->
+    (exists s, ty = embed s) ->
+    embed (unembed ty) = ty.
+  Proof.
+    intros A inj ty eq_dec ex_prf.
+    destruct (eq_dec (embed (unembed ty)) ty) as [ | devil ].
+    - assumption.
+    - assert False; [ | contradiction ].
+      inversion ex_prf as [ s ty_eq ].
+      rewrite ty_eq in devil.
+      rewrite unembedEmbed in devil.
+      apply devil; reflexivity.
+  Qed.
+
+  Lemma embedUnembedClosed:
+    forall `{InjectiveEmbedding EmptySet} (ty: TypeScheme (VariableSymbol := EmptySet)),
+    (exists s, ty = embed s) ->
+    embed (unembed ty) = ty.
+  Proof.
+    intros.
+    apply embedUnembed; [ | assumption ].
+    intros sigma tau.
+    destruct (IntersectionType_eq_dec (freeze sigma) (freeze tau)) as [ eq | not_eq ].
+    - generalize (f_equal (@unfreeze EmptySet)  eq).
+      rewrite freezeUnfreeze.
+      rewrite freezeUnfreeze.
+      intro; left; assumption.
+    - right; intro eq.
+      generalize (f_equal freeze eq).
+      assumption.
+  Qed.
+
+  Lemma embedUnembedOpen:
+    forall `{InjectiveEmbedding VariableSymbol} (ty: TypeScheme (VariableSymbol := VariableSymbol)),
+    (exists s, ty = embed s) ->
+    embed (unembed ty) = ty.
+  Proof.
+    intros.
+    apply embedUnembed; [ exact TypeScheme_eq_dec | assumption ].
+  Qed.
+
+  Class ProperEmbedding :=
+    { EmbedClosed :> InjectiveEmbedding EmptySet;
+      EmbedOpen :> InjectiveEmbedding SigSpec.Var;
+      
+      embed_respectful: forall (s s': Sort EmptySet), subsorts s s' -> freeze (embed s) <= freeze (embed s');
+      unembed_respectful:
+        forall (sigma tau: IntersectionType),
+            (exists s, sigma = freeze (embed s)) -> (exists s, tau = freeze (embed s)) ->
+            sigma <= tau -> subsorts (unembed (unfreeze sigma)) (unembed (unfreeze tau));
+      embed_Path: forall s, Path (freeze (embed s));
+      embedApply: forall S s, freeze (embed (applySubst S s)) = Apply (embedSubst S) (embed s);
+      unembedApply: forall S tau,
+          (exists s, tau = embed s) ->
+          Apply S tau = freeze (embed (applySubst (unembedSubst S) (unembed tau))) }.
   
+  Lemma unembed_embedSubst `{ProperEmbedding}: forall S alpha,
+      unembedSubst (embedSubst S) alpha = S alpha.
+  Proof.
+    intros S alpha.
+    unfold embedSubst.
+    unfold unembedSubst.
+    rewrite (freezeUnfreeze).
+    rewrite unembedEmbed.
+    reflexivity.
+  Qed.
+  Lemma embed_unembedSubst `{ProperEmbedding}: forall S alpha,
+      (exists s, unfreeze (VariableSymbol := EmptySet) (S alpha) = embed s) ->
+      embedSubst (unembedSubst S) alpha = S alpha.
+  Proof.
+    intros S alpha fromSort.
+    unfold embedSubst.
+    unfold unembedSubst.
+    rewrite (embedUnembedClosed _ fromSort).
+    rewrite unfreezeFreeze.
+    reflexivity.
+  Qed.
+End SortEmbedding.
+
+Module Type WithProperEmbedding(SigSpec: CompatibleCLSignature)(Types: IntersectionTypes(SigSpec)).
+  Declare Module Embedding: SortEmbedding(SigSpec)(Types).
+  Export Embedding.
+  Declare Instance ProperlyEmbedded: ProperEmbedding.
+End WithProperEmbedding.
+
+(*
+
 Module Type ProtectedSymbols(SigSpec: CompatibleCLSignature) <: CompatibleCLSignature.
   Definition Sort: Set -> Set := SigSpec.Sort.
   Definition Var: Set := SigSpec.Var.
@@ -135,107 +242,6 @@ Module Type ProtectedSymbols(SigSpec: CompatibleCLSignature) <: CompatibleCLSign
   Definition ClosedSortsInhabited := SigSpec.ClosedSortsInhabited.
   Definition OpenSortsInhabited := SigSpec.OpenSortsInhabited.
 End ProtectedSymbols.
-
-Module Type SortEmbedding(Import SigSpec: CompatibleCLSignature)(Import Types: IntersectionTypes(SigSpec)).
-  Class Embedding (A: Set) :=
-    { embed: Sort A -> TypeScheme (VariableSymbol := A);
-      unembed: TypeScheme (VariableSymbol := A) -> Sort A; }.
-
-  Definition embedSubst `{Embedding EmptySet}: (SigSpec.Var -> Sort EmptySet) -> (SigSpec.Var -> IntersectionType) :=
-    fun S alpha => freeze (embed (S alpha)).
-  Definition unembedSubst `{Embedding EmptySet}: (SigSpec.Var -> IntersectionType) -> (SigSpec.Var -> Sort EmptySet) :=
-    fun S alpha => unembed (unfreeze (S alpha)).
-
-  Class InjectiveEmbedding (A: Set) :=
-    { Embed :> Embedding A;
-      unembedEmbed: forall (s: Sort A), unembed (embed s) = s }.
-
-  Lemma embedUnembed:
-    forall {A: Set} `{InjectiveEmbedding A} (ty: TypeScheme (VariableSymbol := A)),
-    (forall (sigma tau: TypeScheme (VariableSymbol := A)), { sigma = tau } + { sigma <> tau }) ->
-    (exists s, ty = embed s) ->
-    embed (unembed ty) = ty.
-  Proof.
-    intros A inj ty eq_dec ex_prf.
-    destruct (eq_dec (embed (unembed ty)) ty) as [ | devil ].
-    - assumption.
-    - assert False; [ | contradiction ].
-      inversion ex_prf as [ s ty_eq ].
-      rewrite ty_eq in devil.
-      rewrite unembedEmbed in devil.
-      apply devil; reflexivity.
-  Qed.
-
-  Lemma embedUnembedClosed:
-    forall `{InjectiveEmbedding EmptySet} (ty: TypeScheme (VariableSymbol := EmptySet)),
-    (exists s, ty = embed s) ->
-    embed (unembed ty) = ty.
-  Proof.
-    intros.
-    apply embedUnembed; [ | assumption ].
-    intros sigma tau.
-    destruct (IntersectionType_eq_dec (freeze sigma) (freeze tau)) as [ eq | not_eq ].
-    - generalize (f_equal (@unfreeze EmptySet)  eq).
-      rewrite freezeUnfreeze.
-      rewrite freezeUnfreeze.
-      intro; left; assumption.
-    - right; intro eq.
-      generalize (f_equal freeze eq).
-      assumption.
-  Qed.
-
-  Lemma embedUnembedOpen:
-    forall `{InjectiveEmbedding VariableSymbol} (ty: TypeScheme (VariableSymbol := VariableSymbol)),
-    (exists s, ty = embed s) ->
-    embed (unembed ty) = ty.
-  Proof.
-    intros.
-    apply embedUnembed; [ exact TypeScheme_eq_dec | assumption ].
-  Qed.
-
-  Class ProperEmbedding :=
-    { EmbedClosed :> InjectiveEmbedding EmptySet;
-      EmbedOpen :> InjectiveEmbedding SigSpec.Var;
-      
-      embed_respectful: forall (s s': Sort EmptySet), subsorts s s' -> freeze (embed s) <= freeze (embed s');
-      unembed_respectful:
-        forall (sigma tau: IntersectionType),
-            (exists s, sigma = freeze (embed s)) -> (exists s, tau = freeze (embed s)) ->
-            sigma <= tau -> subsorts (unembed (unfreeze sigma)) (unembed (unfreeze tau));
-      embed_Path: forall s, Path (freeze (embed s));
-      embedApply: forall S s, freeze (embed (applySubst S s)) = Apply (embedSubst S) (embed s);
-      unembedApply: forall S tau,
-          (exists s, tau = embed s) ->
-          Apply S tau = freeze (embed (applySubst (unembedSubst S) (unembed tau))) }.
-  
-  Lemma unembed_embedSubst `{ProperEmbedding}: forall S alpha,
-      unembedSubst (embedSubst S) alpha = S alpha.
-  Proof.
-    intros S alpha.
-    unfold embedSubst.
-    unfold unembedSubst.
-    rewrite (freezeUnfreeze).
-    rewrite unembedEmbed.
-    reflexivity.
-  Qed.
-  Lemma embed_unembedSubst `{ProperEmbedding}: forall S alpha,
-      (exists s, unfreeze (VariableSymbol := EmptySet) (S alpha) = embed s) ->
-      embedSubst (unembedSubst S) alpha = S alpha.
-  Proof.
-    intros S alpha fromSort.
-    unfold embedSubst.
-    unfold unembedSubst.
-    rewrite (embedUnembedClosed _ fromSort).
-    rewrite unfreezeFreeze.
-    reflexivity.
-  Qed.
-End SortEmbedding.
-
-Module Type WithProperEmbedding(SigSpec: CompatibleCLSignature)(Types: IntersectionTypes(SigSpec)).
-  Declare Module Embedding: SortEmbedding(SigSpec)(Types).
-  Export Embedding.
-  Declare Instance ProperlyEmbedded: ProperEmbedding.
-End WithProperEmbedding.
 
 Module LiftProperEmbedding
        (SigSpec: CompatibleCLSignature)
@@ -610,6 +616,214 @@ Module LiftProperEmbedding
           assert (tau_eq: tau1 = tau2); [ auto | rewrite tau_eq ].
           reflexivity.
       Qed.
+
+      Lemma liftRespectful: forall (s s': Sort EmptySet), subsorts s s' -> freeze (embed s) <= freeze (embed s').
+      Proof.
+        intros s s' subsorts.
+        unfold embed.
+        unfold ClosedEmbedding.
+        unfold liftEmbed.
+        rewrite liftFreeze.
+        rewrite liftFreeze.
+        apply liftTypeRespectful.
+        apply UnprotectedEmbedding.Embedding.embed_respectful.
+        assumption.
+      Qed.
+        
+
+      Definition unliftSubst (S: Substitution): Types.Substitution :=
+        fun alpha => unliftType' (S alpha).
+
+      Lemma unliftApply_eq: forall S tau,
+          Apply S tau = liftType (Types.Apply (unliftSubst S)
+                                              (match unliftScheme tau with
+                                               | Some ty => ty
+                                               | _ => Types.omegaScheme end)).
+      Proof.
+        intros S tau.
+        induction tau using TypeScheme_rect'.
+        - simpl.
+          unfold unliftSubst.
+          rewrite lift
+          
+
+      Lemma liftUnembedApply: forall S tau,
+          (exists s, tau = embed s) ->
+          Apply S tau = freeze (embed (applySubst (unembedSubst S) (unembed tau))).
+      Proof.
+        intros S tau exprf.
+        generalize (UnprotectedEmbedding.Embedding.
+        
+        unfold unembed.
+        unfold OpenEmbedding.
+        unfold liftUnembed.
+        destruct exprf as [ s tau_eq ].
+        rewrite tau_eq.
+        unfold embed.
+        unfold OpenEmbedding.
+        unfold liftEmbed.
+        rewrite unliftLift.
+        unfold ClosedEmbedding.
+        unfold liftEmbed.
+        rewrite liftFreeze.
+        unfold unembedSubst.
+        unfold unembed.
+        unfold liftUnembed.
+        
+        generalize (UnprotectedEmbedding.Embedding.unembedApply (fun x => unliftType' (S x)) tau).
+        unfold liftScheme.
+        unfold OpenSortsInhabited.
+        
+      
+      Lemma liftEmbedApply: forall S s, freeze (embed (applySubst S s)) = Apply (embedSubst S) (embed s).
+      Proof.
+        intros S s.
+        simpl.
+        unfold embedSubst.
+        unfold liftEmbed.
+        rewrite liftFreeze.
+        rewrite (UnprotectedEmbedding.Embedding.embedApply).
+        destruct (UnprotectedEmbedding.Embedding.embed) as [ | skel ].
+        - simpl.
+          unfold liftEmbed.
+          rewrite liftFreeze.
+          apply f_equal.
+          unfold UnprotectedEmbedding.Embedding.embedSubst.
+          reflexivity.
+        - induction (Types.Skeleton skel)
+            as [ | | C args prfs | | ] using Types.TypeScheme_rect'.
+          + simpl.
+            unfold liftEmbed.
+            rewrite liftFreeze.
+            apply f_equal.
+            unfold UnprotectedEmbedding.Embedding.embedSubst.
+            reflexivity.
+          + reflexivity.
+          + simpl.
+            unfold Const.
+            unfold liftPreType.
+            apply f_equal.
+            apply f_equal.
+            rewrite <- map_fg.
+            rewrite <- map_fg.
+            simpl embed in prfs.
+            generalize (Forall_nth _ _ (ForAll'Forall _ _ prfs)).
+            clear prfs.
+            revert args.
+            simpl.
+            generalize (constructorArity C).
+            intros n args.
+            induction args.
+            * intros; reflexivity.
+            * intro kth_eq.
+              generalize (kth_eq Fin.F1).
+              simpl.
+              intro hd_eq; rewrite hd_eq.
+              apply f_equal.
+              
+            
+   
+
+      Lemma liftEmbed_Path: forall s, Path (freeze (embed s)).
+      Proof.
+        intro s.
+        unfold embed.
+        unfold ClosedEmbedding.
+        unfold liftEmbed.
+        generalize (UnprotectedEmbedding.Embedding.embed_Path s).
+        destruct UnprotectedEmbedding.Embedding.embed as [ | skel ].
+        - contradiction.
+        - induction (Types.Skeleton skel)
+            as [ | | C args IH | | ] using Types.TypeScheme_rect'.
+          + contradiction.
+          + intro pathprf; inversion pathprf.
+          + intro pathprf.
+            simpl in pathprf.
+            apply Path_Const.
+            inversion pathprf as [ ? ? prf [ C_eq args_eq ] | ].
+            dependent rewrite args_eq in prf.
+            clear C_eq args_eq pathprf.
+            revert args IH prf.
+            simpl.
+            generalize (constructorArity C).
+            clear ...
+            intros arity args IH.
+            generalize (Forall_nth _ _ (ForAll'Forall _ _ IH)).
+            clear IH; intro IH'.
+            assert (IH: forall k, Types.Path (nth (map Types.freeze args) k) -> Path (freeze (liftScheme (nth args k)))).
+            { intro k.
+              rewrite (nth_map (Types.freeze) args k _ eq_refl).
+              intro; auto. }
+            clear IH'.
+            intro argsprf; revert IH.
+            inversion argsprf as [ n_eq [ n_eq' args_eq ] | n sigma sigma_path n_eq [n_eq' args_eq] | ].
+            * clear argsprf.
+              revert args args_eq.
+              rewrite <- n_eq.
+              intros args args_eq.
+              intro; simpl.
+              apply (fun r => case0 (fun xs => PathArgs (map _ (map _ xs))) r args).
+              simpl.
+              apply PathArgs_nil.
+            * clear argsprf.
+              revert args args_eq.
+              rewrite <- n_eq.
+              intros args args_eq.
+              assert (tl_omega: map freeze (map liftScheme (tl args)) = const omega n).
+              { revert args_eq.
+                apply (caseS' args); clear args; intros arg args.
+                simpl.
+                clear ...
+                intro args_eq.
+                generalize (vect_exist_eq _ _ args_eq).
+                clear args_eq.
+                intro args_eq'.
+                inversion args_eq' as [ [ sigma_eq args_eq ] ].
+                clear sigma_eq args_eq'.
+                generalize (vect_exist_eq _ _ args_eq).
+                clear args_eq; intro args_eq.
+                induction args as [ | arg' n args IH ].
+                - intros; simpl; reflexivity.
+                - simpl in args_eq.
+                  inversion args_eq as [ [ arg'_eq args_eq' ] ].
+                  generalize (vect_exist_eq _ _ args_eq').
+                  clear args_eq args_eq'.
+                  intro args_eq.
+                  induction arg' using Types.TypeScheme_rect'; inversion arg'_eq; try solve [ contradiction ].
+                  simpl.
+                  apply f_equal.
+                  auto. }
+              assert (hd_path: Path (freeze (liftScheme (hd args)))).
+              { generalize (vect_exist_eq _ _ args_eq).
+                clear args_eq tl_omega.
+                apply (caseS' args); clear args; intros arg args.
+                intro args_eq.
+                simpl.
+                inversion args_eq as [ [ sigma_eq args_eq' ] ].
+                rewrite sigma_eq in sigma_path.
+                revert sigma_path.
+                clear ...
+                induction arg using Types.TypeScheme_rect';
+                  intro path_prf;
+                  inversion path_prf; try solve [contradiction ].
+                - simpl.
+                  
+                
+              apply (caseS' args); clear args; intros arg args.
+              intro IH.
+              simpl.
+              apply PathArgs_cons_arg.
+              
+              
+            
+          + intro pathprf; apply Path_Arr.
+            inversion pathprf.
+            auto.
+          + intro pathprf; inversion pathprf.
+            
+        
+     
+
       
       Definition forall_args_map {A B: Type} (P: B -> B -> Prop) n (sigmas taus: t A n) (f: A -> B)
                (prf: Forall2 P (map f sigmas) (map f taus))
@@ -646,6 +860,8 @@ Module LiftProperEmbedding
                                                                    rew <- [fun xs => Forall2 P xs taus] xs'_eq in
                                                                    prfs))))
            end sigmas eq_refl taus eq_refl) _ _ _ prf.
+
+      
       
       Fixpoint unliftTypeRespectful' sigma tau (prf: liftType sigma <= liftType tau) {struct prf}:
         Types.Subtypes sigma tau.
@@ -765,17 +981,7 @@ Module LiftProperEmbedding
           rewrite (eq_trans (eq_sym C2_eq') C1_eq').
           rewrite (eq_trans (eq_sym C3_eq') C1_eq').
           intros sigmas taus args1 args2 args3 args1_eq args2_eq args3_eq.
-          
-          
-          inversion  C1_eq.
-          inversion C2_eq.
-          revert C2_eq C3_eq.
-          rewrite C1_eq.
-          intro C2_eq.
-          
-          
-          rewrite liftTypeDistrib.
-          apply ST_InterConstDistrib.
+          admit.
         - apply ST_SubtypeDistrib; auto.
         - apply ST_CoContra; auto.
         - apply ST_OmegaTop.
@@ -783,19 +989,8 @@ Module LiftProperEmbedding
         - eapply ST_Trans; eauto.
       Qed.
 
-      Lemma liftRespectful: forall (s s': Sort EmptySet), subsorts s s' -> freeze (embed s) <= freeze (embed s').
-      Proof.
-        intros s s' subsorts.
-        unfold embed.
-        unfold ClosedEmbedding.
-        unfold liftEmbed.
-        rewrite liftFreeze.
-        rewrite liftFreeze.
-        apply liftTypeRespectful.
-        apply UnprotectedEmbedding.Embedding.embed_respectful.
-        assumption.
-      Qed.
-       *)
+      
+       
       Lemma unliftRespectful:
         forall (sigma tau: IntersectionType),
             (exists s, sigma = freeze (embed s)) -> (exists s, tau = freeze (embed s)) ->
@@ -834,503 +1029,523 @@ Module LiftProperEmbedding
     End EmbeddingImpl.
     Instance ProperlyEmbedded: ProperEmbedding.
   End LiftedEmbedding.
-End LiftProperEmbedding.
+End LiftProperEmbedding. *)
 
 Module CombinatoryLogicAlgebra
        (Import SigSpec: CompatibleCLSignature)
-       (Import Logic: CombinatoryLogicSignature(SigSpec))
-       (Import ProperEmbedding: WithProperEmbedding(SigSpec)(Logic)).
-  Context {UnprotectedConstructorSymbol: Set}.
+       (Import Types: IntersectionTypes(SigSpec))
+       (Import Terms: Terms(SigSpec))
+       (Import ProperEmbedding: WithProperEmbedding(SigSpec)(Types))
+       (Import TypesCountable: CountableTypes(SigSpec)(Types))
+       (Import WF: DecidableWellFormedPredicate(SigSpec)(Types))
+       (Import CL: CombinatoryLogic(SigSpec)(Types)(Terms)(WF))
+       (Import CPL: ComputationalPathLemma(SigSpec)(Types)(Terms)(TypesCountable)(WF)(CL))
+       (Import Alg: Algebraic(SigSpec)).
+  (*Context {UnprotectedConstructorSymbol: Set}.
   Context `{Signature: `{SignatureSpecification}}.
   Context `{ContextSymbols: `{SymbolSpecification UnprotectedConstructorSymbol Operation}}.
-  Import ProtectedSymbols.
   Context `{Embedding: `{ProperEmbedding (ContextSymbols := ProtectedSymbolSpecificationInstance)}}.
 
   Implicit Types ConstructorSymbol : (unit + UnprotectedConstructorSymbol).
-  Implicit Types VariableSymbol := Var.
+  Implicit Types VariableSymbol := Var.*)
   
-  Definition blackBoxEmbedOpen (s: Sort Var): TypeScheme (VariableSymbol := Var) :=
-    ConstScheme blackBox (cons _ (embed s) _ (nil _)).
+  Definition blackBoxEmbedOpen (s: Sort SigSpec.Var): TypeScheme (VariableSymbol := SigSpec.Var) :=
+    ConstScheme BlackBox (rew <- BlackBoxArity in cons _ (embed s) _ (nil _)).
 
-  Definition blackBoxEmbed (s: Sort EmptySet): IntersectionType (ConstructorSymbol := unit + ConstructorSymbol) :=
-    freeze (ConstructorSymbol := unit + ConstructorSymbol)  (Skeleton  (ConstructorSymbol := unit + ConstructorSymbol) (PT_Const (ConstructorSymbol := unit + ConstructorSymbol) blackBox (cons _ (embed s) _ (nil _)))).
+  Definition blackBoxEmbed (s: Sort EmptySet): IntersectionType :=
+    freeze (Skeleton (PT_Const BlackBox (rew <- BlackBoxArity in cons _ (embed s) _ (nil _)))).
 
-    Definition Gamma (c: Operation) :=
-      (fix Gamma_rec n dom :=
-         match dom with
-         | nil _ => blackBoxEmbedOpen (range c)
-         | cons _ param _ params =>
-           ArrowScheme (blackBoxEmbedOpen param) (Gamma_rec _ params)
-         end) _ (domain c).
+  Definition Gamma (c: Operation) :=
+    (fix Gamma_rec n dom :=
+       match dom with
+       | nil _ => blackBoxEmbedOpen (range c)
+       | cons _ param _ params =>
+         ArrowScheme (blackBoxEmbedOpen param) (Gamma_rec _ params)
+       end) _ (domain c).
+  
+  Lemma Gamma_paths:
+    forall (c: Operation) (S: SigSpec.Var -> Sort EmptySet),
+      Path (Apply (embedSubst S) (Gamma c)).
+  Proof.
+    intros c S.
+    unfold Gamma.
+    induction (domain c).
+    - unfold blackBoxEmbedOpen.
+      apply Path_Const.
+      simpl.
+      rewrite BlackBoxArity.
+      simpl.
+      apply PathArgs_cons_arg.
+      fold (Apply).
+      rewrite <- embedApply.
+      apply embed_Path.
+    - apply Path_Arr.
+      assumption.
+  Qed.
 
-    Lemma Gamma_paths:
-      forall (c: Operation) (S: Var -> Sort EmptySet),
-        Path (Apply (embedSubst S) (Gamma c)).
-    Proof.
-      intros c S.
-      unfold Gamma.
-      induction (domain c).
-      - unfold blackBoxEmbedOpen.
-        apply Path_Const.
-        simpl.
-        apply PathArgs_cons_arg.
-        fold (Apply).
-        rewrite <- embedApply.
-        apply embed_Path.
-      - apply Path_Arr.
-        assumption.
-    Qed.
+  Lemma source_count_eq : forall S op, src_count (Apply (embedSubst S) (Gamma op)) = arity op.
+  Proof.
+    intros S op.
+    unfold Gamma.
+    generalize (arity op) (domain op).
+    intros arity domain.
+    induction domain as [ | ? ? ? IH ].
+    - reflexivity.
+    - simpl.
+      rewrite IH.
+      reflexivity.
+  Qed. 
 
-    Lemma source_count_eq : forall S op, src_count (Apply (embedSubst S) (Gamma op)) = arity op.
-    Proof.
-      intros S op.
-      unfold Gamma.
-      generalize (arity op) (domain op).
-      intros arity domain.
-      induction domain as [ | ? ? ? IH ].
-      - reflexivity.
-      - simpl.
-        rewrite IH.
-        reflexivity.
-    Qed. 
+  Definition Carrier s := { M : Term | CL Gamma M (blackBoxEmbed s) }.
 
-    Definition Carrier s := { M : Term | CL Gamma M (blackBoxEmbed s) }.
+  Definition ProjectTerms: forall S n (args: t (Sort SigSpec.Var) n),
+      F_args Carrier S args -> t Term n :=
+    fun S n args f => 
+      map (fun k => proj1_sig ((F_args_nth _ _ _ f) k)) (positions n).
 
-    Definition ProjectTerms: forall S n (args: t (Sort Signature.Var) n),
-        F_args Sort Carrier S args -> t Term n :=
-      fun S n args f => 
-        map (fun k => proj1_sig ((F_args_nth _ _ _ _ f) k)) (positions n).
-
-    Lemma blackBoxEmbed_nth:
-      forall op S k (src_count_eq: src_count (Apply (embedSubst S) (Gamma op)) = arity op),
-        blackBoxEmbed (applySubst S (nth (domain op) (rew <- eq_sym src_count_eq in k))) =
-        nth
-          (fst
-             (split_path (Apply (embedSubst S) (Gamma op)) (src_count (Apply (embedSubst S) (Gamma op)))
-                         (le_n (src_count (Apply (embedSubst S) (Gamma op)))))) k.
-    Proof.
-      intros op S k src_count_eq.
-      generalize (le_n (src_count (Apply (embedSubst S) (Gamma op)))).
-      revert k.
-      generalize src_count_eq.
-      match goal with
-      | [ |- ?tgt ] =>
-        apply (fun x =>
+  Lemma blackBoxEmbed_nth:
+    forall op S k (src_count_eq: src_count (Apply (embedSubst S) (Gamma op)) = arity op),
+      blackBoxEmbed (applySubst S (nth (domain op) (rew <- eq_sym src_count_eq in k))) =
+      nth
+        (fst
+           (split_path (Apply (embedSubst S) (Gamma op)) (src_count (Apply (embedSubst S) (Gamma op)))
+                       (le_n (src_count (Apply (embedSubst S) (Gamma op)))))) k.
+  Proof.
+    intros op S k src_count_eq.
+    generalize (le_n (src_count (Apply (embedSubst S) (Gamma op)))).
+    revert k.
+    generalize src_count_eq.
+    match goal with
+    | [ |- ?tgt ] =>
+      apply (fun x =>
                rew <- [fun n =>
-                      forall (src_count_eq: n = arity op)
-                        (k: Fin.t n)
-                        (prf: (n <= src_count (Apply (embedSubst S) (Gamma op)))%nat),
-                        blackBoxEmbed (applySubst S (nth (domain op) (rew <- [Fin.t] eq_sym src_count_eq in k))) =
-                        nth (fst (split_path (Apply (embedSubst S) (Gamma op)) n prf)) k]
+                        forall (src_count_eq: n = arity op)
+                          (k: Fin.t n)
+                          (prf: (n <= src_count (Apply (embedSubst S) (Gamma op)))%nat),
+                          blackBoxEmbed (applySubst S (nth (domain op) (rew <- [Fin.t] eq_sym src_count_eq in k))) =
+                          nth (fst (split_path (Apply (embedSubst S) (Gamma op)) n prf)) k]
                    (src_count_eq) in x)
-      end.
-      clear src_count_eq.
-      intros src_count_eq k prf.
-      unfold eq_rect_r.
-      rewrite <- (eq_rect_eq_dec (Nat.eq_dec) _ _ (eq_sym _)).
-      clear src_count_eq.
-      apply (Forall2_nth (fun x y => blackBoxEmbed (applySubst S x) = y)
-                         (domain op)
-                         (fst (split_path (Apply (embedSubst S) (Gamma op)) (arity op) prf))).
-      clear k.
-      revert prf.
-      unfold Gamma.
-      induction (domain op) as [ | ? ? ? IH ].
-      - intros; apply Forall2_nil.
-      - intro prf. 
-        apply Forall2_cons.
-        + unfold blackBoxEmbed.
-          unfold blackBoxEmbedOpen.
-          simpl.
-          apply f_equal.
-          rewrite embedApply.
-          reflexivity.
-        + apply IH.
-    Qed.
-    
-    Definition CL_Algebra:
-      forall (WellFormed : (Signature.Var -> Sort EmptySet) -> Prop),
-        (forall S, WellFormed S -> TypeSystem.WellFormed (embedSubst S)) ->
-        SigmaAlgebra Sort Signature.Var subsorts WellFormed Carrier.
-    Proof.
-      unfold SigmaAlgebra.
-      intros WF WF_transport s Fs.
-      destruct Fs as [ op S WF_S args tgt_le ].
-      assert (opty : CL Gamma (Symbol op) (Apply (embedSubst S) (Gamma op))).
-      { apply CL_Var.
-        apply WF_transport; assumption. }
-      generalize (source_count_eq S op).
-      intro source_count_eq.
-      assert (args' :
-        { Ns: t Term (src_count (Apply (embedSubst S) (Gamma op)))
-        | Forall2 (CL Gamma) Ns (fst (split_path (Apply (embedSubst S) (Gamma op))
-                                                 (src_count (Apply (embedSubst S) (Gamma op)))
-                                                 (le_n _))) }).
-      { exists (rew <- source_count_eq in ProjectTerms _ _ _ args).
-        apply nth_Forall2.
-        unfold eq_rect_r.
-        intro k.
-        assert (rew_ext:
-            (rew [fun n => t Term n] eq_sym source_count_eq in (ProjectTerms S (arity op) (domain op) args)) =
-            rew [t Term] eq_sym source_count_eq in (ProjectTerms S (arity op) (domain op) args)).
-        { rewrite <- (eq_sym source_count_eq).
-          simpl.
-          reflexivity. }
-        rewrite rew_ext.
-        rewrite (nth_k (eq_sym source_count_eq) (ProjectTerms S (arity op) (domain op) args) k).
-        unfold ProjectTerms.
-        rewrite (nth_map _ _ _ _ eq_refl).
-        rewrite (positions_spec).
-        destruct (F_args_nth _ _ _ _ args (rew <- [Fin.t] eq_sym source_count_eq in k)) as [ M proof ].        
+    end.
+    clear src_count_eq.
+    intros src_count_eq k prf.
+    unfold eq_rect_r.
+    rewrite <- (eq_rect_eq_dec (Nat.eq_dec) _ _ (eq_sym _)).
+    clear src_count_eq.
+    apply (Forall2_nth (fun x y => blackBoxEmbed (applySubst S x) = y)
+                       (domain op)
+                       (fst (split_path (Apply (embedSubst S) (Gamma op)) (arity op) prf))).
+    clear k.
+    revert prf.
+    unfold Gamma.
+    induction (domain op) as [ | ? ? ? IH ].
+    - intros; apply Forall2_nil.
+    - intro prf. 
+      apply Forall2_cons.
+      + unfold blackBoxEmbed.
+        unfold blackBoxEmbedOpen.
         simpl.
-        rewrite <- (blackBoxEmbed_nth _ _ _ source_count_eq).
-        assumption. }
-      clear args.
-      assert (tgt_le':
-          snd (split_path (Apply (embedSubst S) (Gamma op))
-                          (src_count (Apply (embedSubst S) (Gamma op)))
-                          (le_n _)) <= blackBoxEmbed s).
-      { unfold blackBoxEmbed.
-        simpl freeze.
-        unfold Gamma.
-        clear args'.
-        generalize (domain op).
-        rewrite <- source_count_eq.
-        clear source_count_eq.
-        intro domain.
-        induction domain as [ | ? ? ? IH ].
-        - simpl.
-          apply (ST_Ax _ _ eq_refl); [ reflexivity | ].
-          apply Forall2_cons; [ | apply Forall2_nil ].
-          rewrite <- embedApply.
-          apply embed_respectful.
-          assumption.
-        - simpl.
-          match goal with
-          | [ |- (snd (split_path _ _ ?prfSx) <= _)] =>
-            rewrite (split_path_proof_invariant _ _ _ prfSx) in IH
-          end.
-          exact IH. }
-      eexists.
-      eapply CL_ST; [ | apply tgt_le' ].
-      eapply CL_ApplyPath.
-      - apply Gamma_paths. 
-      - eassumption.
-      - exact (proj2_sig args').
-    Defined.
-
-    Lemma unembedApply_c: forall S c,
-        Apply (embedSubst (unembedSubst S)) (Gamma c) =
-        Apply S (Gamma c).
-    Proof.
-      intros S c.
+        apply f_equal.
+        rewrite BlackBoxArity.
+        simpl.
+        rewrite embedApply.
+        reflexivity.
+      + apply IH.
+  Qed.
+  
+  Definition CL_Algebra:
+      (forall S, SigSpec.WellFormed S -> WF.WellFormed (embedSubst S)) ->
+      SigmaAlgebra Carrier.
+  Proof.
+    unfold SigmaAlgebra.
+    intros WF_transport s Fs.
+    destruct Fs as [ op S WF_S args tgt_le ].
+    assert (opty : CL Gamma (Symbol op) (Apply (embedSubst S) (Gamma op))).
+    { apply CL_Var.
+      apply WF_transport; assumption. }
+    generalize (source_count_eq S op).
+    intro source_count_eq.
+    assert (args' :
+              { Ns: t Term (src_count (Apply (embedSubst S) (Gamma op)))
+              | Forall2 (CL Gamma) Ns (fst (split_path (Apply (embedSubst S) (Gamma op))
+                                                       (src_count (Apply (embedSubst S) (Gamma op)))
+                                                       (le_n _))) }).
+    { exists (rew <- source_count_eq in ProjectTerms _ _ _ args).
+      apply nth_Forall2.
+      unfold eq_rect_r.
+      intro k.
+      assert (rew_ext:
+                (rew [fun n => t Term n] eq_sym source_count_eq in (ProjectTerms S (arity op) (domain op) args)) =
+                rew [t Term] eq_sym source_count_eq in (ProjectTerms S (arity op) (domain op) args)).
+      { rewrite <- (eq_sym source_count_eq).
+        simpl.
+        reflexivity. }
+      rewrite rew_ext.
+      rewrite (nth_k (eq_sym source_count_eq) (ProjectTerms S (arity op) (domain op) args) k).
+      unfold ProjectTerms.
+      rewrite (nth_map _ _ _ _ eq_refl).
+      rewrite (positions_spec).
+      destruct (F_args_nth _ _ _ args (rew <- [Fin.t] eq_sym source_count_eq in k)) as [ M proof ].        
+      simpl.
+      rewrite <- (blackBoxEmbed_nth _ _ _ source_count_eq).
+      assumption. }
+    clear args.
+    assert (tgt_le':
+              snd (split_path (Apply (embedSubst S) (Gamma op))
+                              (src_count (Apply (embedSubst S) (Gamma op)))
+                              (le_n _)) <= blackBoxEmbed s).
+    { unfold blackBoxEmbed.
+      simpl freeze.
       unfold Gamma.
-      induction (domain c) as [ | ? ? ? IH ].
-      - unfold blackBoxEmbedOpen.
-        simpl Apply.
-        apply f_equal.
-        match goal with
-        |[|- cons _ ?lhs _ _ = cons _ ?rhs _ _] =>
-         assert (s_eq: lhs = rhs)
-        end.
-        { match goal with
-          |[|- _ = Apply S ?erc ] =>
-           assert (ex_s: exists s, erc = embed s); [ eexists; reflexivity | ];
-             rewrite (unembedApply S _ ex_s)
-          end.
-          rewrite <- embedApply.
-          rewrite unembedEmbed.
-          reflexivity. }
-        rewrite s_eq.
-        reflexivity.
+      clear args'.
+      generalize (domain op).
+      rewrite <- source_count_eq.
+      clear source_count_eq.
+      intro domain.
+      induction domain as [ | ? ? ? IH ].
       - simpl.
-        apply (f_equal2); [ | exact IH ].
-        apply f_equal.
+        apply (ST_Ax _ _ eq_refl); [ reflexivity | ].
+        rewrite BlackBoxArity.
+        apply Forall2_cons; [ | apply Forall2_nil ].
+        rewrite <- embedApply.
+        apply embed_respectful.
+        assumption.
+      - simpl.
         match goal with
-        |[|- cons _ ?lhs _ _ = cons _ ?rhs _ _] =>
-         assert (s_eq: lhs = rhs)
+        | [ |- (snd (split_path _ _ ?prfSx) <= _)] =>
+          rewrite (split_path_proof_invariant _ _ _ prfSx) in IH
         end.
-        { match goal with
-          |[|- _ = Apply S ?erc ] =>
-           assert (ex_s: exists s, erc = embed s); [ eexists; reflexivity | ];
-             rewrite (unembedApply S _ ex_s)
-          end.
-          rewrite <- embedApply.
+        exact IH. }
+    eexists.
+    eapply CL_ST; [ | apply tgt_le' ].
+    eapply CL_ApplyPath.
+    - apply Gamma_paths. 
+    - eassumption.
+    - exact (proj2_sig args').
+  Defined.
+
+  Lemma unembedApply_c: forall S c,
+      Apply (embedSubst (unembedSubst S)) (Gamma c) =
+      Apply S (Gamma c).
+  Proof.
+    intros S c.
+    unfold Gamma.
+    induction (domain c) as [ | ? ? ? IH ].
+    - unfold blackBoxEmbedOpen.
+      simpl Apply.
+      apply f_equal.
+      rewrite BlackBoxArity.
+      simpl.
+      match goal with
+      |[|- cons _ ?lhs _ _ = cons _ ?rhs _ _] =>
+       assert (s_eq: lhs = rhs)
+      end.
+      { match goal with
+        |[|- _ = Apply S ?erc ] =>
+         assert (ex_s: exists s, erc = embed s); [ eexists; reflexivity | ];
+           rewrite (unembedApply S _ ex_s)
+        end.
+        rewrite <- embedApply.
+        rewrite unembedEmbed.
+        reflexivity. }
+      rewrite s_eq.
+      reflexivity.
+    - simpl.
+      apply (f_equal2); [ | exact IH ].
+      apply f_equal.
+      rewrite BlackBoxArity.
+      simpl.
+      match goal with
+      |[|- cons _ ?lhs _ _ = cons _ ?rhs _ _] =>
+       assert (s_eq: lhs = rhs)
+      end.
+      { match goal with
+        |[|- _ = Apply S ?erc ] =>
+         assert (ex_s: exists s, erc = embed s); [ eexists; reflexivity | ];
+           rewrite (unembedApply S _ ex_s)
+        end.
+        rewrite <- embedApply.
+        rewrite unembedEmbed.
+        reflexivity. }
+      rewrite s_eq.
+      reflexivity.
+  Qed.
+
+  Definition CL_CoAlgebra:
+      (forall S, WF.WellFormed S -> SigSpec.WellFormed (unembedSubst S)) ->
+      (forall M sigma, {CL Gamma M sigma} + {CL Gamma M sigma -> False}) ->
+      SigmaCoAlgebra Carrier.
+  Proof.
+    intros WF_transport CL_dec.
+    unfold SigmaCoAlgebra.
+    intros s prf.
+    destruct prf as [ M prf ].
+    assert (path_s : Path (blackBoxEmbed s)).
+    { unfold blackBoxEmbed.
+      apply Path_Const.
+      simpl.
+      rewrite BlackBoxArity.
+      simpl.
+      apply PathArgs_cons_arg.
+      fold freeze.
+      apply embed_Path. }
+    generalize (CL_Path_path _ _ _ prf path_s).
+    intro ex_subst.
+    generalize (CL_Path_path_compute_S _ CL_dec _ _ path_s ex_subst).
+    clear ex_subst; intro ex_subst.
+    assert (fully_applied: argumentCount M = arity (rootOf M)).
+    { destruct ex_subst as [ S [ WF_S ex_path ] ].
+      unfold CombinatorSymbol.
+      rewrite <- (source_count_eq (unembedSubst S) (rootOf M)).
+      rewrite unembedApply_c.
+      generalize (ST_organize_ge (Apply S (Gamma (rootOf M)))).
+      rewrite (factorize_organized _ (organize_organized _)).
+      induction ex_path as [ ? ? ? here | ? x xs ].
+      - destruct here as [ path_x [ argCountPrf [ _ tgt_le ] ] ].
+        intro x_ge.
+        rewrite (ST_intersect_nth _ Fin.F1) in x_ge.
+        simpl in x_ge.
+        generalize (Gamma_paths (rootOf M) (unembedSubst S)).
+        rewrite unembedApply_c.
+        intro path_c.
+        generalize (Path_src_count _ _ x_ge path_c path_x).
+        intro src_count_eq'.
+        rewrite src_count_eq'.
+        inversion argCountPrf as [ | n argCountPrf' src_count_eq'' ].
+        + reflexivity.
+        + assert (argCountPrf'' : (Datatypes.S (argumentCount M) <= Datatypes.S n)%nat).
+          { rewrite <- Nat.succ_le_mono.
+            assumption. }
+          rewrite src_count_eq'' in argCountPrf''.
+          generalize (split_path_step _ _ argCountPrf argCountPrf'').
+          intro split_path_eq.
+          rewrite split_path_eq in tgt_le.
+          unfold blackBoxEmbed in tgt_le.
+          assert False; [ | contradiction ].
+          apply (ST_Arrow_Const _ _ _ _ tgt_le).
+      - rewrite (ST_intersect_append_le (cons _ x _ (nil _)) xs).
+        rewrite (ST_InterMeetRight).
+        intro; auto. }
+    apply (mkF _ _ (rootOf M) (unembedSubst (proj1_sig ex_subst)));
+      destruct ex_subst as [ S [ WF_S ex_path ] ].
+    - apply WF_transport; assumption.
+    - generalize (ST_organize_ge (Apply S (Gamma (rootOf M)))).
+      simpl.
+      rewrite (factorize_organized _ (organize_organized (Apply S (Gamma (rootOf M))))).
+      intro root_le.
+      apply nth_F_args.
+      intro k.
+      set (k' := rew <- fully_applied in k).
+      exists (nth (argumentsOf M) k').
+      induction ex_path as [ ? x ? here | ? x xs ? IH ].
+      + destruct here as [ path_x [ argCountPrf [ args_inhab tgt_le ] ] ].
+        eapply CL_ST.
+        * apply (Forall2_nth _ _ _ args_inhab k').
+        * generalize (Gamma_paths (rootOf M) (unembedSubst S)).
+          rewrite unembedApply_c.
+          intro path_c.
+          rewrite (ST_intersect_nth _ Fin.F1) in root_le.
+          assert (argCountPrf' : (argumentCount M <= src_count (Apply S (Gamma (rootOf M))))%nat).
+          { generalize (Path_src_count _ _ root_le path_c path_x).
+            intro count_eq.
+            rewrite count_eq.
+            assumption. }               
+          generalize (Forall2_nth _ _ _ (ST_path_src_n _ _ path_c path_x root_le _ argCountPrf' argCountPrf) k').
+          intro arg_le.
+          rewrite arg_le.
+          unfold Gamma.
+          clear arg_le.
+          revert fully_applied k' argCountPrf'.
+          clear ...
+          intro fully_applied.
+          rewrite fully_applied.
+          unfold eq_rect_r.
+          simpl.
+          clear fully_applied.
+          unfold Gamma.
+          fold CombinatorSymbol in k.
+          fold CombinatorSymbol.
+          induction (domain (rootOf M)) as [ | ? ? ? IH ].
+          { inversion k. }
+          { intro argCountPrf.
+            apply (Fin.caseS' k).
+            - simpl.
+              unfold blackBoxEmbed.
+              simpl.
+              apply (ST_Ax _ _ eq_refl); [ reflexivity | ].
+              rewrite BlackBoxArity.
+              simpl.
+              rewrite unembedApply; [ | eexists; reflexivity ].
+              unfold eq_rect_r.
+              simpl.
+              rewrite unembedEmbed.
+              apply Forall2_cons; [ | apply Forall2_nil ].
+              reflexivity.
+            - intro k'.
+              apply (IH k' (proj2 (Nat.succ_le_mono _ _) argCountPrf)). }
+      + rewrite (ST_intersect_append_le (cons _ x _ (nil _)) xs) in root_le.
+        rewrite (ST_InterMeetRight) in root_le.
+        auto.
+    - assert (source_count_le : (arity (rootOf M) <= src_count (Apply S (Gamma (rootOf M))))%nat).
+      { generalize (source_count_eq (unembedSubst S) (rootOf M)).
+        intro source_count_eq.
+        rewrite unembedApply_c in source_count_eq.
+        unfold CombinatorSymbol.
+        rewrite <- source_count_eq.
+        reflexivity. }
+      assert (split_path_eq:
+                snd (split_path (Apply S (Gamma (rootOf M))) _ source_count_le) =
+                blackBoxEmbed (applySubst (unembedSubst S) (range (rootOf M)))).
+      { clear ...
+        revert source_count_le.
+        generalize (rootOf M).
+        clear M.
+        intros c.
+        unfold Gamma.
+        unfold blackBoxEmbed.
+        fold CombinatorSymbol.
+        induction (domain c) as [ | ? ? ? IH ].
+        - intros; simpl.
+          apply f_equal.
+          rewrite BlackBoxArity.
+          simpl.
+          rewrite unembedApply; [ | eexists; reflexivity ].
           rewrite unembedEmbed.
-          reflexivity. }
-        rewrite s_eq.
-        reflexivity.
-    Qed.
+          reflexivity.
+        - simpl.
+          intro source_count_le.
+          generalize (proj2 (PeanoNat.Nat.succ_le_mono _ _) source_count_le).
+          intro source_count_le'.
+          generalize (IH source_count_le').
+          intro IH'.
+          exact IH'. }
+      assert (path_tgt_le:
+                snd (split_path (Apply S (Gamma (rootOf M))) _ source_count_le) <=
+                blackBoxEmbed s).
+      { generalize (ST_organize_ge (Apply S (Gamma (rootOf M)))).
+        rewrite (factorize_organized _ (organize_organized _)).
+        induction ex_path as [ ? ? ? here | ? x xs there IH ].
+        - intro x_ge.
+          rewrite (ST_intersect_nth _ Fin.F1) in x_ge.
+          simpl in x_ge.
+          destruct here as [ path_x [ argCountPrf [ inhab_args x_tgt_le ] ] ].
+          rewrite <- x_tgt_le.
+          generalize (Gamma_paths (rootOf M) (unembedSubst S)).
+          rewrite unembedApply_c.
+          intro path_c.
+          clear split_path_eq inhab_args x_tgt_le.
+          revert fully_applied source_count_le path_c path_x x_ge argCountPrf.
+          clear ...
+          intros fully_applied source_count_le path_c path_x x_ge.
+          rewrite fully_applied.
+          intro argCountPrf.            
+          apply (ST_path_tgt_n _ _ path_c path_x x_ge _ _ argCountPrf).
+        - intro xs_ge.
+          rewrite (ST_intersect_append_le (cons _ x _ (nil _)) xs) in xs_ge.
+          rewrite (ST_InterMeetRight _ _) in xs_ge.
+          exact (IH xs_ge). }
+      rewrite split_path_eq in path_tgt_le.
+      unfold blackBoxEmbed in path_tgt_le.
+      simpl in path_tgt_le.
+      generalize (CI_complete _ _ _ path_tgt_le).
+      intro path_tgt_ci.
+      inversion path_tgt_ci as [ ? ? arity_eq ? args_st [ hd_eq tl_eq ] | | | ].
+      unfold eq_rect_r in args_st.
+      rewrite <- (eq_rect_eq_dec (Nat.eq_dec) _ _ (eq_sym arity_eq)) in args_st.
+      rewrite (vect_exist_eq _ _
+                             (existT_fg_eq (fun x => t IntersectionType x) constructorArity _ _ _ tl_eq))
+        in args_st.
+      rewrite BlackBoxArity in args_st.
+      simpl in args_st.
+      inversion args_st as [ | ? ? ? ? ? arg_st ].
+      generalize (unembed_respectful _ _
+                                     (ex_intro _ _ eq_refl)
+                                     (ex_intro _ _ eq_refl)
+                                     arg_st).
+      intro arg_subsorts.
+      rewrite freezeUnfreeze in arg_subsorts.
+      rewrite freezeUnfreeze in arg_subsorts.
+      rewrite unembedEmbed in arg_subsorts.
+      rewrite unembedEmbed in arg_subsorts.
+      exact arg_subsorts.
+  Defined.
 
-    Definition CL_CoAlgebra:
-      forall (WellFormed : (Signature.Var -> Sort EmptySet) -> Prop),
-        (forall S, TypeSystem.WellFormed S -> WellFormed (unembedSubst S)) ->
-        (forall S, { TypeSystem.WellFormed S } + { TypeSystem.WellFormed S -> False }) ->
-        (forall M sigma, {CL Gamma M sigma} + {CL Gamma M sigma -> False}) ->
-        SigmaCoAlgebra Sort Signature.Var subsorts WellFormed Carrier.
-     Proof.
-       intros WF WF_transport WF_dec CL_dec.
-       unfold SigmaCoAlgebra.
-       intros s prf.
-       destruct prf as [ M prf ].
-       assert (path_s : Path (blackBoxEmbed s)).
-       { unfold blackBoxEmbed.
-         apply Path_Const.
-         simpl.
-         apply PathArgs_cons_arg.
-         fold freeze.
-         apply embed_Path. }
-       generalize (CL_Path_path _ _ _ prf path_s).
-       intro ex_subst.
-       generalize (CL_Path_path_compute_S WF_dec _ CL_dec _ _ path_s ex_subst).
-       clear ex_subst; intro ex_subst.
-       assert (fully_applied: argumentCount M = arity (rootOf M)).
-       { destruct ex_subst as [ S [ WF_S ex_path ] ].
-         rewrite <- (source_count_eq (unembedSubst S) (rootOf M)).
-         rewrite unembedApply_c.
-         generalize (ST_organize_ge (Apply S (Gamma (rootOf M)))).
-         rewrite (factorize_organized _ (organize_organized _)).
-         induction ex_path as [ ? ? ? here | ? x xs ].
-         - destruct here as [ path_x [ argCountPrf [ _ tgt_le ] ] ].
-           intro x_ge.
-           rewrite (ST_intersect_nth _ Fin.F1) in x_ge.
-           simpl in x_ge.
-           generalize (Gamma_paths (rootOf M) (unembedSubst S)).
-           rewrite unembedApply_c.
-           intro path_c.
-           generalize (Path_src_count _ _ x_ge path_c path_x).
-           intro src_count_eq'.
-           rewrite src_count_eq'.
-           inversion argCountPrf as [ | n argCountPrf' src_count_eq'' ].
-           + reflexivity.
-           + assert (argCountPrf'' : (Datatypes.S (argumentCount M) <= Datatypes.S n)%nat).
-             { rewrite <- Nat.succ_le_mono.
-               assumption. }
-             rewrite src_count_eq'' in argCountPrf''.
-             generalize (split_path_step _ _ argCountPrf argCountPrf'').
-             intro split_path_eq.
-             rewrite split_path_eq in tgt_le.
-             unfold blackBoxEmbed in tgt_le.
-             assert False; [ | contradiction ].
-             apply (ST_Arrow_Const _ _ _ _ tgt_le).
-         - rewrite (ST_intersect_append_le (cons _ x _ (nil _)) xs).
-           rewrite (ST_InterMeetRight).
-           intro; auto. }
-       apply (mkF _ _ _ _ _ _ (rootOf M) (unembedSubst (proj1_sig ex_subst)));
-         destruct ex_subst as [ S [ WF_S ex_path ] ].
-       - apply WF_transport; assumption.
-       - generalize (ST_organize_ge (Apply S (Gamma (rootOf M)))).
-         simpl.
-         rewrite (factorize_organized _ (organize_organized (Apply S (Gamma (rootOf M))))).
-         intro root_le.
-         apply nth_F_args.
-         intro k.
-         set (k' := rew <- fully_applied in k).
-         exists (nth (argumentsOf M) k').
-         induction ex_path as [ ? x ? here | ? x xs ? IH ].
-         + destruct here as [ path_x [ argCountPrf [ args_inhab tgt_le ] ] ].
-           eapply CL_ST.
-           * apply (Forall2_nth _ _ _ args_inhab k').
-           * generalize (Gamma_paths (rootOf M) (unembedSubst S)).
-             rewrite unembedApply_c.
-             intro path_c.
-             rewrite (ST_intersect_nth _ Fin.F1) in root_le.
-             assert (argCountPrf' : (argumentCount M <= src_count (Apply S (Gamma (rootOf M))))%nat).
-             { generalize (Path_src_count _ _ root_le path_c path_x).
-               intro count_eq.
-               rewrite count_eq.
-               assumption. }               
-             generalize (Forall2_nth _ _ _ (ST_path_src_n _ _ path_c path_x root_le _ argCountPrf' argCountPrf) k').
-             intro arg_le.
-             rewrite arg_le.
-             unfold Gamma.
-             clear arg_le.
-             revert fully_applied k' argCountPrf'.
-             clear ...
-             intro fully_applied.
-             rewrite fully_applied.
-             unfold eq_rect_r.
-             simpl.
-             clear fully_applied.
-             unfold Gamma.
-             induction (domain (rootOf M)) as [ | ? ? ? IH ].
-             { inversion k. }
-             { intro argCountPrf.
-               apply (Fin.caseS' k).
-               - simpl.
-                 unfold blackBoxEmbed.
-                 simpl.
-                 rewrite unembedApply; [ | eexists; reflexivity ].
-                 apply (ST_Ax _ _ eq_refl); [ reflexivity | ].
-                 unfold eq_rect_r.
-                 simpl.
-                 rewrite unembedEmbed.
-                 apply Forall2_cons; [ | apply Forall2_nil ].
-                 reflexivity.
-               - intro k'.
-                 apply (IH k' (proj2 (Nat.succ_le_mono _ _) argCountPrf)). }
-         + rewrite (ST_intersect_append_le (cons _ x _ (nil _)) xs) in root_le.
-           rewrite (ST_InterMeetRight) in root_le.
-           auto.
-       - assert (source_count_le : (arity (rootOf M) <= src_count (Apply S (Gamma (rootOf M))))%nat).
-         { generalize (source_count_eq (unembedSubst S) (rootOf M)).
-           intro source_count_eq.
-           rewrite unembedApply_c in source_count_eq.
-           rewrite <- source_count_eq.
-           reflexivity. }
-         assert (split_path_eq:
-           snd (split_path (Apply S (Gamma (rootOf M))) _ source_count_le) =
-           blackBoxEmbed (applySubst (unembedSubst S) (range (rootOf M)))).
-         { clear ...
-           revert source_count_le.
-           generalize (rootOf M).
-           clear M.
-           intros c.
-           unfold Gamma.
-           unfold blackBoxEmbed.
-           induction (domain c) as [ | ? ? ? IH ].
-           - intros; simpl.
-             rewrite unembedApply; [ | eexists; reflexivity ].
-             rewrite unembedEmbed.
-             reflexivity.
-           - simpl.
-             intro source_count_le.
-             generalize (proj2 (PeanoNat.Nat.succ_le_mono _ _) source_count_le).
-             intro source_count_le'.
-             generalize (IH source_count_le').
-             intro IH'.
-             exact IH'. }
-         assert (path_tgt_le:
-           snd (split_path (Apply S (Gamma (rootOf M))) _ source_count_le) <=
-           blackBoxEmbed s).
-         { generalize (ST_organize_ge (Apply S (Gamma (rootOf M)))).
-           rewrite (factorize_organized _ (organize_organized _)).
-           induction ex_path as [ ? ? ? here | ? x xs there IH ].
-           - intro x_ge.
-             rewrite (ST_intersect_nth _ Fin.F1) in x_ge.
-             simpl in x_ge.
-             destruct here as [ path_x [ argCountPrf [ inhab_args x_tgt_le ] ] ].
-             rewrite <- x_tgt_le.
-             generalize (Gamma_paths (rootOf M) (unembedSubst S)).
-             rewrite unembedApply_c.
-             intro path_c.
-             clear split_path_eq inhab_args x_tgt_le.
-             revert fully_applied source_count_le path_c path_x x_ge argCountPrf.
-             clear ...
-             intros fully_applied source_count_le path_c path_x x_ge.
-             rewrite fully_applied.
-             intro argCountPrf.            
-             apply (ST_path_tgt_n _ _ path_c path_x x_ge _ _ argCountPrf).
-           - intro xs_ge.
-             rewrite (ST_intersect_append_le (cons _ x _ (nil _)) xs) in xs_ge.
-             rewrite (ST_InterMeetRight _ _) in xs_ge.
-             exact (IH xs_ge). }
-         rewrite split_path_eq in path_tgt_le.
-         unfold blackBoxEmbed in path_tgt_le.
-         simpl in path_tgt_le.
-         generalize (CI_complete _ _ _ path_tgt_le).
-         intro path_tgt_ci.
-         inversion path_tgt_ci as [ ? ? arity_eq ? args_st [ hd_eq tl_eq ] | | | ].
-         unfold eq_rect_r in args_st.
-         rewrite <- (eq_rect_eq_dec (Nat.eq_dec) _ _ (eq_sym arity_eq)) in args_st.
-         rewrite (vect_exist_eq _ _
-                                 (existT_fg_eq (fun x => t IntersectionType x) constructorArity _ _ _ tl_eq))
-           in args_st.
-         inversion args_st as [ | ? ? ? ? ? arg_st ].
-         generalize (unembed_respectful _ _
-                                        (ex_intro _ _ eq_refl)
-                                        (ex_intro _ _ eq_refl)
-                                        arg_st).
-         intro arg_subsorts.
-         rewrite freezeUnfreeze in arg_subsorts.
-         rewrite freezeUnfreeze in arg_subsorts.
-         rewrite unembedEmbed in arg_subsorts.
-         rewrite unembedEmbed in arg_subsorts.
-         exact arg_subsorts.
-     Defined.
+  Definition carrier_eq: forall s s', Carrier s -> Carrier s' -> Prop :=
+    fun s1 s2 c1 c2 => proj1_sig c1 = proj1_sig c2.
 
-     Definition carrier_eq: forall s s', Carrier s -> Carrier s' -> Prop :=
-       fun s1 s2 c1 c2 => proj1_sig c1 = proj1_sig c2.
+  Lemma carrier_eq_refl: forall s c, carrier_eq s s c c.
+  Proof.
+    intros; reflexivity.
+  Qed.
+  Lemma carrier_eq_sym: forall s s' c1 c2, carrier_eq s s' c1 c2 -> carrier_eq s' s c2 c1.
+  Proof.
+    intros; apply eq_sym; assumption.
+  Qed.
+  Lemma carrier_eq_trans: forall s s' s'' c1 c2 c3,
+      carrier_eq s s' c1 c2 -> carrier_eq s' s'' c2 c3 -> carrier_eq s s'' c1 c3.
+  Proof.
+    intros; eapply eq_trans; eassumption.
+  Qed.
 
-     Lemma carrier_eq_refl: forall s c, carrier_eq s s c c.
-     Proof.
-       intros; reflexivity.
-     Qed.
-     Lemma carrier_eq_sym: forall s s' c1 c2, carrier_eq s s' c1 c2 -> carrier_eq s' s c2 c1.
-     Proof.
-       intros; apply eq_sym; assumption.
-     Qed.
-     Lemma carrier_eq_trans: forall s s' s'' c1 c2 c3,
-         carrier_eq s s' c1 c2 -> carrier_eq s' s'' c2 c3 -> carrier_eq s s'' c1 c3.
-     Proof.
-       intros; eapply eq_trans; eassumption.
-     Qed.
+  Lemma CL_Algebra_op:
+    forall (WF_transport: forall S, SigSpec.WellFormed S -> WF.WellFormed (embedSubst S)),
+    forall s f, rootOf (proj1_sig (CL_Algebra WF_transport s f)) = op _ _ f.
+  Proof.
+    intros WF_transport s f.
+    unfold CL_Algebra.
+    destruct f as [ op subst wf args tgt_le ].
+    simpl.
+    rewrite (applyAllRoot).
+    reflexivity.
+  Qed.
+  
+  Lemma CL_Algebra_argCount:
+    forall (WF_transport: forall S, SigSpec.WellFormed S -> WF.WellFormed (embedSubst S)),
+    forall s f, argumentCount (proj1_sig (CL_Algebra WF_transport s f)) =
+           (arity (op _ _ f)).
+  Proof.
+    intros WF_transport s f.
+    unfold CL_Algebra.
+    destruct f as [ op subst wf args tgt_le ].
+    simpl.
+    rewrite (applyAllArgumentCount).
+    simpl.
+    rewrite (source_count_eq).
+    reflexivity.
+  Defined.
 
-     Lemma CL_Algebra_op:
-       forall (WellFormed : (Signature.Var -> Sort EmptySet) -> Prop)
-         (WF_transport: forall S, WellFormed S -> TypeSystem.WellFormed (embedSubst S)),
-       forall s f, rootOf (proj1_sig (CL_Algebra WellFormed WF_transport s f)) = op _ _ _ _ _ _ f.
-     Proof.
-       intros WF WF_transport s f.
-       unfold CL_Algebra.
-       destruct f as [ op subst wf args tgt_le ].
-       simpl.
-       rewrite (applyAllRoot).
-       reflexivity.
-     Qed.
-     
-     Lemma CL_Algebra_argCount:
-       forall (WellFormed : (Signature.Var -> Sort EmptySet) -> Prop)
-         (WF_transport: forall S, WellFormed S -> TypeSystem.WellFormed (embedSubst S)),
-       forall s f, argumentCount (proj1_sig (CL_Algebra WellFormed WF_transport s f)) =
-              (arity (op _ _ _ _ _ _ f)).
-     Proof.
-       intros WF WF_transport s f.
-       unfold CL_Algebra.
-       destruct f as [ op subst wf args tgt_le ].
-       simpl.
-       rewrite (applyAllArgumentCount).
-       simpl.
-       rewrite (source_count_eq).
-       reflexivity.
-     Defined.
+  Lemma CL_Algebra_args:
+    forall (WF_transport: forall S, SigSpec.WellFormed S -> WF.WellFormed (embedSubst S)),
+    forall s f, argumentsOf (proj1_sig (CL_Algebra WF_transport s f)) =
+           rew <- (CL_Algebra_argCount WF_transport s f) in ProjectTerms _ _ _ (args _ _ f).
+  Proof.
+    intros WF_transport s f.
+    destruct f as [ op subst wf args tgt_le ].       
+    simpl.
+    rewrite (applyAllArguments).
+    simpl.
+    match goal with
+      [|- (rew <- [t Term] ?prf1 in rew <- [t Term] ?prf2 in _) =
+         (rew <- [t Term] ?prf3 in _) ] =>
+      generalize prf2 prf1 prf3
+    end.
+    intro prf1.
+    rewrite prf1.
+    unfold eq_rect_r.
+    simpl.
+    intros prf2 prf3.
+    rewrite (UIP_dec (Nat.eq_dec) prf2 prf3).
+    reflexivity.
+  Qed.
 
-     Lemma CL_Algebra_args:
-       forall (WellFormed : (Signature.Var -> Sort EmptySet) -> Prop)
-         (WF_transport: forall S, WellFormed S -> TypeSystem.WellFormed (embedSubst S)),
-       forall s f, argumentsOf (proj1_sig (CL_Algebra WellFormed WF_transport s f)) =
-              rew <- (CL_Algebra_argCount WellFormed WF_transport s f) in ProjectTerms _ _ _ (args _ _ _ _ _ _ f).
-     Proof.
-       intros WF WF_transport s f.
-       destruct f as [ op subst wf args tgt_le ].       
-       simpl.
-       rewrite (applyAllArguments).
-       simpl.
-       match goal with
-         [|- (rew <- [t Term] ?prf1 in rew <- [t Term] ?prf2 in _) =
-            (rew <- [t Term] ?prf3 in _) ] =>
-         generalize prf2 prf1 prf3
-       end.
-       intro prf1.
-       rewrite prf1.
-       unfold eq_rect_r.
-       simpl.
-       intros prf2 prf3.
-       rewrite (UIP_dec (Nat.eq_dec) prf2 prf3).
-       reflexivity.
-     Qed.
-
-     Lemma CL_CoAlgebra_op:
-       forall (WellFormed : (Signature.Var -> Sort EmptySet) -> Prop)
-         (WF_transport: forall S, TypeSystem.WellFormed S -> WellFormed (unembedSubst S))
-         (WF_dec: forall S, { TypeSystem.WellFormed S } + { TypeSystem.WellFormed S -> False })
-         (CL_dec: forall M sigma, {CL Gamma M sigma} + {CL Gamma M sigma -> False}),
-       forall s c, op _ _ _ _ _ _ (CL_CoAlgebra WellFormed WF_transport WF_dec CL_dec s c) = rootOf (proj1_sig c).
-     Proof.
-       intros WF WF_transport WF_dec CL_dec s c.
-       destruct c as [ M prf ].
-       reflexivity.
-     Qed.
+  Lemma CL_CoAlgebra_op:
+    forall (WF_transport: forall S, WF.WellFormed S -> SigSpec.WellFormed (unembedSubst S))
+      (CL_dec: forall M sigma, {CL Gamma M sigma} + {CL Gamma M sigma -> False}),
+    forall s c, op _ _ (CL_CoAlgebra WF_transport  CL_dec s c) = rootOf (proj1_sig c).
+  Proof.
+    intros WF_transport CL_dec s c.
+    destruct c as [ M prf ].
+    reflexivity.
+  Qed.
 (*
      Lemma CL_CoAlgebra_arity:
        forall (WellFormed : (Signature.Var -> Sort EmptySet) -> Prop)
@@ -1384,6 +1599,6 @@ Module CombinatoryLogicAlgebra
          revert alg.
          induction (arity).
          + simpl in alg.
-     *)
-  End Algebra.
-End CLAlgebra.*)
+ *)
+
+End CombinatoryLogicAlgebra.
