ComputationalPathLemma.v
@@ -1,4 +1,3 @@
-Require Import Coq.Logic.ConstructiveEpsilon.
 Require Import Coq.Classes.RelationClasses.
 Require Import Coq.Arith.PeanoNat.
 Require Import Coq.Lists.List.
@@ -15,6 +14,7 @@ Require Import VectorQuantification.
 Require Import CombinatoryLogic.
 Require Import IntersectionTypes.
 Require Import CombinatoryTerm.
+Require Import ConstructiveExtensionalEpsilon.
 Require Import Cantor.
 
 Import EqNotations.
@@ -26,11 +26,265 @@ Module Type CountableTypeSignature <: TypeSignature.
   Declare Instance Variables_finite: Finite VariableSymbol.
 End CountableTypeSignature.
 
+Module Type CountableTypes
+       (Import Signature: CountableTypeSignature)
+       (Import Types: IntersectionTypes.IntersectionTypes Signature).
+
+  Definition vectToNat {A: Set} (toNat: A -> nat) {n: nat} (xs: t A n): nat :=
+    (fix vectToNat_rec (n: nat) (xs: t A n): nat :=
+       match xs with
+       | nil _ => 0
+       | cons _ x n xs => cantor_pair (toNat x) (vectToNat_rec _ xs)
+       end) _ xs.
+  
+  Fixpoint typeToNat_rec (tau: IntersectionType): nat :=
+    match tau with
+    | Ty (PT_omega) => cantor_sum (inl 0)
+    | Ty (PT_Const C args) =>
+      cantor_sum (* omega + ... *)
+        (inr (cantor_sum (* const + ... *)
+                (inl (cantor_pair (toNat C) (vectToNat typeToNat_rec args)))))
+    | Ty (PT_Arrow sigma tau) =>
+      cantor_sum (* omega + ... *)
+        (inr (cantor_sum (* const + ... *)
+                (inr (cantor_sum (* arrow + inter *)
+                        (inl (cantor_pair (typeToNat_rec sigma) (typeToNat_rec tau)))))))
+    | Ty (PT_Inter sigma tau) =>
+      cantor_sum (* omega + ... *)
+        (inr (cantor_sum (* const + ... *)
+                (inr (cantor_sum (* arrow + inter *)
+                        (inr (cantor_pair (typeToNat_rec sigma) (typeToNat_rec tau)))))))
+    end.
+
+  Fixpoint fuelForType (tau: IntersectionType): nat :=
+    match tau with
+    | Ty (PT_omega) => 1
+    | Ty (PT_Const C args) => 1 + (fold_right (Nat.max) (map fuelForType args) 0)
+    | Ty (PT_Arrow sigma tau) => 1 + (Nat.max (fuelForType sigma) (fuelForType tau))
+    | Ty (PT_Inter sigma tau) => 1 + (Nat.max (fuelForType sigma) (fuelForType tau))
+    end.
+
+  Definition typeToNat (tau: IntersectionType): nat :=
+    cantor_pair (fuelForType tau) (typeToNat_rec tau).
+  
+  Definition vectFromNat {A: Set} (fromNat: nat -> A) (m: nat) (n: nat): t A m :=
+    (fix vectFromNat_rec m n: t A m :=
+       match m with
+       | 0 => nil _
+       | S m => cons _ (fromNat (fst (cantor_pair_inv n))) _
+                    (vectFromNat_rec m (snd (cantor_pair_inv n)))
+       end) m n.
+
+  Fixpoint natToType_rec (fuel n: nat): IntersectionType :=
+    match fuel with
+    | 0 => omega
+    | S fuel =>
+      match cantor_sum_inv n with
+      | inl _ => omega
+      | inr n =>
+        match cantor_sum_inv n with
+        | inl n =>
+          Const (fromNat (fst (cantor_pair_inv n)))
+                (vectFromNat (natToType_rec fuel) _ (snd (cantor_pair_inv n)))
+        | inr n =>
+          match cantor_sum_inv n with
+          | inl n =>
+            Arrow (natToType_rec fuel (fst (cantor_pair_inv n)))
+                  (natToType_rec fuel (snd (cantor_pair_inv n)))
+          | inr n =>
+            Inter (natToType_rec fuel (fst (cantor_pair_inv n)))
+                  (natToType_rec fuel (snd (cantor_pair_inv n)))
+          end
+        end
+      end
+    end.
+  
+  Definition natToType (n: nat): IntersectionType :=
+     natToType_rec (fst (cantor_pair_inv n)) (snd (cantor_pair_inv n)).
+
+  Lemma omega_inj: forall fuel, natToType_rec fuel (typeToNat_rec omega) = omega.
+  Proof.
+    intro fuel.
+    destruct fuel; reflexivity.
+  Qed.
+
+  Lemma arrow_inj:
+    forall sigma tau
+      (IH_sigma: forall fuel, fuel >= fuelForType sigma -> natToType_rec fuel (typeToNat_rec sigma) = sigma)
+      (IH_tau: forall fuel, fuel >= fuelForType tau -> natToType_rec fuel (typeToNat_rec tau) = tau)
+      fuel,
+      fuel >= S (Nat.max (fuelForType sigma) (fuelForType tau)) ->
+      natToType_rec fuel (typeToNat_rec (Arrow sigma tau)) = Arrow sigma tau.
+  Proof.
+    intros sigma tau IH_sigma IH_tau fuel max_prf.
+    destruct fuel.
+    - inversion max_prf.
+    - unfold typeToNat_rec.
+      unfold Arrow.
+      unfold liftPreType.
+      unfold natToType_rec.
+      rewrite cantor_sum_inj.
+      rewrite cantor_sum_inj.
+      rewrite cantor_sum_inj.
+      rewrite <- cantor_pair_inj.
+      generalize (IH_sigma fuel (Nat.le_trans _ _ _  (Nat.le_max_l _ _)
+                                              (proj2 (Nat.succ_le_mono _ _) max_prf))).
+      generalize (IH_tau fuel (Nat.le_trans _ _ _  (Nat.le_max_r _ _)
+                                            (proj2 (Nat.succ_le_mono _ _) max_prf))).
+      intros tau_eq sigma_eq.
+      fold (typeToNat_rec sigma).
+      fold (typeToNat_rec tau).
+      fold (natToType_rec fuel (fst (typeToNat_rec sigma, typeToNat_rec tau))).
+      fold (natToType_rec fuel (snd (typeToNat_rec sigma, typeToNat_rec tau))).
+      unfold fst.
+      unfold snd.
+      rewrite sigma_eq.
+      rewrite tau_eq.
+      reflexivity.
+  Qed.
+
+  Lemma inter_inj:
+    forall sigma tau
+      (IH_sigma: forall fuel, fuel >= fuelForType sigma -> natToType_rec fuel (typeToNat_rec sigma) = sigma)
+      (IH_tau: forall fuel, fuel >= fuelForType tau -> natToType_rec fuel (typeToNat_rec tau) = tau)
+      fuel,
+      fuel >= S (Nat.max (fuelForType sigma) (fuelForType tau)) ->
+      natToType_rec fuel (typeToNat_rec (Inter sigma tau)) = Inter sigma tau.
+  Proof.
+    intros sigma tau IH_sigma IH_tau fuel max_prf.
+    destruct fuel.
+    - inversion max_prf.
+    - unfold typeToNat_rec.
+      unfold Inter.
+      unfold liftPreType.
+      unfold natToType_rec.
+      rewrite cantor_sum_inj.
+      rewrite cantor_sum_inj.
+      rewrite cantor_sum_inj.
+      rewrite <- cantor_pair_inj.
+      generalize (IH_sigma fuel (Nat.le_trans _ _ _  (Nat.le_max_l _ _)
+                                              (proj2 (Nat.succ_le_mono _ _) max_prf))).
+      generalize (IH_tau fuel (Nat.le_trans _ _ _  (Nat.le_max_r _ _)
+                                            (proj2 (Nat.succ_le_mono _ _) max_prf))).
+      intros tau_eq sigma_eq.
+      fold (typeToNat_rec sigma).
+      fold (typeToNat_rec tau).
+      fold (natToType_rec fuel (fst (typeToNat_rec sigma, typeToNat_rec tau))).
+      fold (natToType_rec fuel (snd (typeToNat_rec sigma, typeToNat_rec tau))).
+      unfold fst.
+      unfold snd.
+      rewrite sigma_eq.
+      rewrite tau_eq.
+      reflexivity.
+  Qed.
+
+  Lemma vect_inj:
+    forall (A: Set) n (xs: t A n) (fromNat: nat -> A) (toNat: A -> nat)
+      (IH: Forall (fun x => fromNat (toNat x) = x) xs),
+      vectFromNat fromNat n (vectToNat toNat xs) = xs.
+  Proof.
+    intros A n xs fromNat toNat prfs.
+    induction prfs as [ | n x xs prf prfs IH ].
+    - reflexivity.
+    - unfold vectToNat.
+      unfold vectFromNat.
+      rewrite <- cantor_pair_inj.
+      unfold fst.
+      unfold snd.
+      rewrite prf.
+      apply f_equal.
+      apply IH.
+  Qed.
+
+  Lemma ctor_inj:
+    forall C (args: t IntersectionType (constructorArity C))
+      (IH: ForAll' (fun arg => forall fuel, fuel >= fuelForType arg -> natToType_rec fuel (typeToNat_rec arg) = arg) args)
+      fuel,
+      fuel >= 1 + (fold_right (Nat.max) (map fuelForType args) 0) ->
+      natToType_rec fuel (typeToNat_rec (Const C args)) = Const C args.
+  Proof.
+    intros C args IH fuel max_prf.
+    destruct fuel.
+    - inversion max_prf.
+    - assert (args_inj: Forall (fun arg => natToType_rec fuel (typeToNat_rec arg) = arg) args).
+      { apply nth_Forall.
+        generalize (proj2 (Nat.succ_le_mono _ _) max_prf); clear max_prf; intro max_prf.
+        intro k.
+        apply (Forall_nth _ _ (ForAll'Forall _ _ IH) k fuel).
+        clear IH.
+        eapply (Nat.le_trans); [ | apply max_prf].
+        rewrite <- (nth_map fuelForType _ _ _ eq_refl).
+        simpl.
+        clear max_prf.
+        generalize 0.
+        induction k as [ | arity k IH ].
+        - intro s.
+          apply (caseS' args); clear args; intros arg args.
+          simpl.
+          apply Nat.le_max_l.
+        - intro s.
+          apply (caseS' args); clear args; intros arg args.
+          simpl.
+          rewrite (IH args s).
+          apply Nat.le_max_r. }
+      unfold typeToNat_rec.
+      unfold Const.
+      unfold liftPreType.
+      unfold natToType_rec.
+      rewrite cantor_sum_inj.
+      rewrite cantor_sum_inj.
+      rewrite <- cantor_pair_inj.
+      unfold fst.
+      rewrite fromTo_id.
+      unfold snd.
+      fold (typeToNat_rec).
+      generalize (vect_inj _ _ _ _ _ args_inj).
+      intro args_eq.
+      unfold natToType_rec in args_eq.
+      rewrite <- args_eq at 2.
+      unfold Const.
+      unfold liftPreType.
+      reflexivity.
+  Qed.
+
+  Lemma natType_rec_inj:
+    forall tau fuel, fuel >= fuelForType tau -> natToType_rec fuel (typeToNat_rec tau) = tau.
+  Proof.
+    intro tau.
+    induction tau using IntersectionType_rect'.
+    - intros; apply omega_inj.
+    - intros; apply ctor_inj; assumption.
+    - intros; apply arrow_inj; assumption.
+    - intros; apply inter_inj; assumption.
+  Qed.
+
+  Lemma natType_inj:
+    forall tau, natToType (typeToNat tau) = tau.
+  Proof.
+    intro tau.
+    unfold typeToNat.
+    unfold natToType.
+    rewrite <- cantor_pair_inj.
+    simpl fst.
+    simpl snd.
+    apply natType_rec_inj.
+    unfold ge.
+    reflexivity.
+  Qed.
+
+  Instance TypesCountable : `{Countable IntersectionType} :=
+    {| toNat := typeToNat;
+       fromNat := natToType;
+       fromTo_id := natType_inj |}.
+  
+End CountableTypes.
+
 Module Type DecidableWellFormedPredicate
        (Signature: TypeSignature)
        (Import Types: IntersectionTypes.IntersectionTypes Signature) <: WellFormedPredicate(Signature)(Types).
   Include WellFormedPredicate(Signature)(Types).  
-  Parameter WF_dec: forall S, { WellFormed S } + { ~ WellFormed S }.  
+  Parameter WF_dec: forall S, { WellFormed S } + { ~ WellFormed S }.
+  Parameter WF_ext: forall S S', (forall alpha, S alpha = S' alpha) -> WellFormed S -> WellFormed S'.
 End DecidableWellFormedPredicate.
 
 Module Type CountableTypeAndTermSignature := CountableTypeSignature <+ TermSignature.
@@ -39,10 +293,26 @@ Module Type ComputationalPathLemma
        (Import TypesAndTermsSig: CountableTypeAndTermSignature)
        (Import Types: IntersectionTypes.IntersectionTypes(TypesAndTermsSig))
        (Import Terms: CombinatoryTerm.Terms(TypesAndTermsSig))
+       (Import TypesCountable: CountableTypes(TypesAndTermsSig)(Types))
        (Import WF: DecidableWellFormedPredicate(TypesAndTermsSig)(Types))
        (Import CL: CombinatoryLogic(TypesAndTermsSig)(Types)(Terms)(WF)).
-  (* TODO: Show me *)
-  Axiom SubstitutionSpace_countable: `{Countable Substitution}. 
+
+  Definition SubstToNat (S: Substitution): nat :=
+    cantor_fin_fun _ (fun alpha => toNat (S (fromFin alpha))).
+
+  Definition natToSubst (n: nat): Substitution :=
+    fun alpha => fromNat (cantor_fin_fun_inv _ n (toFin alpha)).
+
+  Lemma natSubst_inj: forall S alpha, natToSubst (SubstToNat S) alpha = S alpha.
+  Proof.
+    intros S alpha.
+    unfold natToSubst.
+    unfold SubstToNat.
+    rewrite <- cantor_fin_fun_ext_inj.
+    rewrite fromTo_id.
+    rewrite fromToFin_id.
+    reflexivity.
+  Qed.
   
   Lemma WF_and_le_path_dec: forall sigma_pre sigma S,
       { WellFormed S /\ Apply S sigma_pre <= sigma } + { WellFormed S /\ Apply S sigma_pre <= sigma -> False }.
@@ -199,9 +469,15 @@ Module Type ComputationalPathLemma
         generalize (Forall_nth _ _ prfs F1).
         intros h_prf tl_prfs.
         apply ForAll'_cons.
-        + eapply (constructive_indefinite_ground_description).
-          * apply (fromTo_id).
+        + eapply (constructive_extensional_indefinite_ground_description).
+          * apply natSubst_inj.
           * apply S_sufficient_dec.
+          * intros S S' S_eq wf_exists.
+            destruct wf_exists as [ WF exprf ].
+            split.
+            { eapply WF_ext; eassumption. }
+            { rewrite <- (Apply_ext _ _ S_eq).
+              assumption. }
           * assumption.
         + auto.
     Qed.
@@ -230,9 +506,15 @@ Module Type ComputationalPathLemma
         }.
     Proof.
       intros M sigma path_sigma ex_S.
-      eapply (constructive_indefinite_ground_description).
-      - apply (fromTo_id).
+      eapply (constructive_extensional_indefinite_ground_description).
+      - apply natSubst_inj.
       - apply S_sufficient_dec.
+      - intros S S' S_eq wf_exists.
+        destruct wf_exists as [ WF exprf ].
+        split.
+        + eapply WF_ext; eassumption.
+        + rewrite <- (Apply_ext _ _ S_eq).
+          assumption.
       - assumption.
     Qed.
   End TypeCheckable.
