ConstructiveExtensionalEpsilon.v
@@ -1,0 +1,38 @@
+Require Import Coq.Logic.ConstructiveEpsilon.
+
+Section ConstructiveExtensionalGroundEpsilon.
+
+  Variable A B : Type.
+  Variable f : (A -> B) -> nat.
+  Variable g : nat -> (A -> B).
+
+  Hypothesis gof_eq_id : forall (h : A -> B) (x: A), g (f h) x = h x.
+
+  Variable P : (A -> B) -> Prop.
+  Hypothesis P_decidable : forall h : A -> B, {P h} + {~ P h}.
+  Hypothesis P_extensional: forall h h', (forall x, h x = h' x) -> P h -> P h'.
+
+  Definition P' (x : nat) : Prop := P (g x).
+
+  Lemma P'_decidable : forall n : nat, {P' n} + {~ P' n}.
+  Proof.
+    unfold P'.
+    intro n.
+    apply P_decidable.
+  Qed.
+    
+  Lemma constructive_extensional_indefinite_ground_description : (exists h : A -> B, P h) -> {h : A -> B | P h}.
+  Proof.
+    intro exprf.
+    assert (exn: exists n, P' n).
+    { destruct exprf as [ h Ph ].
+      exists (f h).
+      unfold P'.
+      apply (P_extensional h).
+      - intro x; apply eq_sym; apply gof_eq_id.
+      - assumption. }
+    destruct (constructive_indefinite_ground_description_nat _ P'_decidable exn) as [ n P'n ].
+    exists (g n); exact P'n.
+  Qed.
+
+End ConstructiveExtensionalGroundEpsilon.
